syntax, reduction and declarative typing rules for dependent sums

theories/AutoSubst/PiUniv.sig
@@ -14,3 +14,8 @@ tNatElim : (bind term in term) -> term -> term -> term -> term
 
 tEmpty : term
 tEmptyElim : (bind term in term) -> term -> term
+
+tSig : term -> (bind term in term) -> term
+tPair : term -> (bind term in term) -> term -> term -> term
+tFst : term -> term
+tSnd : term -> term
